NuLLReps.thy
@@ -2,98 +2,79 @@ theory NuLLReps
   imports NuPrim  "HOL-Library.Word"
 begin
 
-instantiation unit :: register_collection begin
-definition layout_unit :: "unit itself \<Rightarrow> layout" where
-  layout_unit_def[simp]: "layout_unit _ = la_z"
-instance by standard
-end
-
-instantiation register :: (llty) register_collection begin
-definition register_unit :: "'a register itself \<Rightarrow> layout" where
-  register_unit_def[simp]: "register_unit _ = la_z"
-instance by standard
-end
-
-instantiation prod :: (llty,llty) llty begin
-definition layout_prod :: "('a \<times> 'b) itself \<Rightarrow> layout" where
-  layout_prod_def[simp]: "layout_prod _ = la_C (layout TYPE('a)) (layout TYPE('b))"
-instance by standard
-end
-
-instantiation prod :: (register_collection,register_collection) register_collection
-  begin instance by standard end
 
   \<comment> \<open> StateOn stack registers
-    where stack :: llty and registers :: register_collection \<close>
+    where stack :: lrep and registers :: register_collection \<close>
 
-instantiation state :: (llty) llty begin
-definition layout_state :: "'a state itself \<Rightarrow> layout" where
-  layout_state_def[simp]: "layout_state _ = la_z"
+instantiation state :: (lrep) lrep begin
+definition llty_state :: "'a state itself \<Rightarrow> llty" where [simp]: "llty_state _ = la_z"
 instance by standard
 end
 
-instantiation with_registers :: (llty,register_collection) llty begin
-definition layout_with_registers :: "('a with 'r) itself \<Rightarrow> layout" where
-  layout_with_registers_def[simp]: "layout_with_registers _ = layout (TYPE ('a))"
+instantiation proc_ctx :: (lrep,register_collection) lrep begin
+definition llty_proc_ctx :: "('a \<flower> 'r) itself \<Rightarrow> llty" where [simp]: "llty_proc_ctx _ = llty (TYPE ('a))"
 instance by standard
 end
 
-instantiation word :: (len) masharable_llty
+instantiation word :: (len) naive_lrep
 begin
-definition layout_word :: "'a word itself \<Rightarrow> layout" where
-  layout_word_def[simp]: "layout_word _ = la_i LENGTH('a)"
-definition share_word :: "'a word \<Rightarrow> zint \<Rightarrow> 'a word" where
-  share_word_def: "share_word x z = x"
-definition sharable_word :: "'a word \<Rightarrow> bool" where
-  sharable_word_def: "sharable_word x = True"
-definition revert_word :: "'a word \<times> 'a word \<Rightarrow> bool" where
-  revert_word_def: "revert_word xy = True"
-definition dpriv_word :: "'a word \<Rightarrow> 'a word" where
-  depriv_word_def: "dpriv_word x = x"
-instance by standard (auto simp add: share_word_def simp add: sharable_word_def
-      simp add: revert_word_def simp add: depriv_word_def)
+definition llty_word :: "'a word itself \<Rightarrow> llty" where [simp]: "llty_word _ = la_i LENGTH('a)"
+definition share_word :: "'a word \<Rightarrow> zint \<Rightarrow> 'a word" where [simp]: "share_word x z = x"
+definition sharable_word :: "'a word \<Rightarrow> bool" where [simp]: "sharable_word x = True"
+definition revert_word :: "'a word \<times> 'a word \<Rightarrow> bool" where [simp]: "revert_word xy = True"
+definition dpriv_word :: "'a word \<Rightarrow> 'a word" where [simp]: "dpriv_word x = x"
+instance by standard auto
 end
 
-instantiation word :: (len) zero_llty
+instantiation word :: (len) zero_lrep
 begin
-definition lty_zero_word[simp]: "lty_zero_word = (0 :: 'a word)"
+definition [simp]: "lty_zero_word = (0 :: 'a word)"
 instance by standard
 end
 
-instantiation word :: (len) ceq_llty
+instantiation word :: (len) ceq_lrep
 begin
-definition ceqable_word :: "'a word \<times> 'a word \<Rightarrow> bool" where
-  ceqable_word_def[simp]: "ceqable_word x = True"
-definition ceq_word :: "'a word \<times> 'a word \<Rightarrow> bool" where
-  ceq_word_def: "ceq_word = (\<lambda>(x,y). (x = y))"
-lemma ceq_word[simp]: "ceq (x,y) = (x = y)" for x :: "'a word"
-   by (simp add: ceq_word_def)
+definition ceqable_word :: "'a word \<times> 'a word \<Rightarrow> bool" where [simp]: "ceqable_word x = True"
+definition ceq_word :: "'a word \<times> 'a word \<Rightarrow> bool" where [simp]: "ceq_word = (\<lambda>(x,y). (x = y))"
+lemma ceq_word[simp]: "ceq (x,y) = (x = y)" for x :: "'a word" by simp
 instance by standard (auto+)
 end
 
-instantiation prod :: (zero_llty, zero_llty) zero_llty begin
-definition lty_zero_prod :: "'a \<times> 'b" where
-  lty_zero_prod_def[simp]: "lty_zero_prod = (lty_zero,lty_zero)"
+instantiation prod :: (zero_lrep, zero_lrep) zero_lrep begin
+definition lty_zero_prod :: "'a \<times> 'b" where [simp]: "lty_zero_prod = (lty_zero,lty_zero)"
 instance by standard
 end
 
-(* declare [[show_hyps = true, show_types = true, show_sorts = true]] *)
-instantiation prod :: (sharable_llty, sharable_llty) sharable_llty begin
-fun revert_prod :: "('a \<times> 'b) \<times> ('a \<times> 'b) \<Rightarrow> bool" where
-  "revert_prod (v1,v2) \<longleftrightarrow> (case v1 of (a1,b1) \<Rightarrow> case v2 of (a2,b2) \<Rightarrow> revert (a1,a2) \<and> revert (b1,b2))"
-fun sharable_prod :: "'a \<times> 'b \<Rightarrow> bool" where
-  "sharable_prod (a,b) \<longleftrightarrow> sharable a \<and> sharable b"
-definition share_prod :: "'a \<times> 'b \<Rightarrow> zint \<Rightarrow> 'a \<times> 'b" where
-  share_prod_def[simp]: "share_prod x z = (case x of (a,b) \<Rightarrow> (share a z, share b z))"
-definition dpriv_prod :: "'a \<times> 'b \<Rightarrow> 'a \<times> 'b" where
-  dpriv_prod_def[simp]: "dpriv_prod x = (case x of (a,b) \<Rightarrow> (dpriv a, dpriv b))"
+instantiation prod :: (sharable_lrep, sharable_lrep) sharable_lrep begin
+definition revert_prod :: "('a \<times> 'b) \<times> ('a \<times> 'b) \<Rightarrow> bool"
+  where "revert_prod v \<longleftrightarrow> (case v of (v1,v2) \<Rightarrow> case v1 of (a1,b1) \<Rightarrow> case v2 of (a2,b2) \<Rightarrow> revert (a1,a2) \<and> revert (b1,b2))"
+lemma [simp]: "revert (v1,v2) \<longleftrightarrow> (case v1 of (a1,b1) \<Rightarrow> case v2 of (a2,b2) \<Rightarrow> revert (a1,a2) \<and> revert (b1,b2))"
+  unfolding revert_prod_def by simp
+definition sharable_prod :: "'a \<times> 'b \<Rightarrow> bool" where "sharable_prod ab \<longleftrightarrow> (case ab of (a,b) \<Rightarrow> sharable a \<and> sharable b)"
+lemma [simp]: "sharable (a,b) \<longleftrightarrow> sharable a \<and> sharable b" unfolding sharable_prod_def by simp
+definition share_prod :: "'a \<times> 'b \<Rightarrow> zint \<Rightarrow> 'a \<times> 'b" where [simp]: "share_prod x z = (case x of (a,b) \<Rightarrow> (share a z, share b z))"
+definition dpriv_prod :: "'a \<times> 'b \<Rightarrow> 'a \<times> 'b" where [simp]: "dpriv_prod x = (case x of (a,b) \<Rightarrow> (dpriv a, dpriv b))"
 instance by standard (auto, (metis revert_sym revert_trans) +)
 end
 
-definition NuNat :: "('a::len) itself \<Rightarrow> ('a word, nat) nu" where
-  NuNat_def: "NuNat _ = Nu (\<lambda>px. case px of (p,x) \<Rightarrow> (p = Word.of_nat x))"
+instantiation prod :: (naive_lrep, naive_lrep) naive_lrep
+  begin instance by standard auto end
 
-lemma NuNat_abst_ex[abst_expn]: "p \<nuLinkL> NuNat b \<nuLinkR> x \<equiv> (p = Word.of_nat x)"
-  by (auto simp add: NuNat_def simp add: abstraction_def)
+instantiation prod :: (ceq_lrep, ceq_lrep) ceq_lrep begin
+definition ceqable_prod :: "('a \<times> 'b) \<times> 'a \<times> 'b \<Rightarrow> bool"
+  where [simp]: "ceqable_prod x = (case x of ((a1,b1),(a2,b2)) \<Rightarrow> ceqable (a1,a2) \<and> ceqable (b1,b2))"
+definition ceq_prod :: "('a \<times> 'b) \<times> 'a \<times> 'b \<Rightarrow> bool"
+  where [simp]: "ceq_prod x = (case x of ((a1,b1),(a2,b2)) \<Rightarrow> ceq (a1,a2) \<and> ceq (b1,b2))"
+instance by standard (auto simp add: ac_simps intro: ceq_trans)
+end
+
+definition NuNat :: "('a::len) itself \<Rightarrow> ('a word, nat) nu"
+  where "NuNat _ = Nu (\<lambda>px. case px of (p,x) \<Rightarrow> (p = Word.of_nat x))"
+syntax "_NuNat_" :: "type \<Rightarrow> logic" (\<open>\<nat>'[_']\<close>)
+translations "\<nat>['x]" == "CONST NuNat (TYPE('x))" 
+lemma [typing_expn]: "p \<nuLinkL> NuNat b \<nuLinkR> x \<equiv> (p = Word.of_nat x)" unfolding NuNat_def by auto
+definition NuBool :: "(1 word, bool) nu" ("\<bool>")
+  where "NuBool = Nu (\<lambda>px. case px of (p,x) \<Rightarrow> (p = 1) = x)"
+lemma [simp]: "p \<nuLinkL> \<bool> \<nuLinkR> x \<longleftrightarrow> (p = 1) = x" unfolding NuBool_def by simp
 
 end
