NuPrim.thy
@@ -2,12 +2,16 @@
 
 theory NuPrim
   imports Main
-  abbrevs "is" = "\<B_i>\<B_s>"
-      and "register" = "\<B_r>\<B_e>\<B_g>\<B_i>\<B_s>\<B_t>\<B_e>\<B_r>"
-      and "in" = "\<B_i>\<B_n>"
-      and "with" = "\<B_w>\<B_i>\<B_t>\<B_h>"
-      and "auxiliary_facts" = "\<B_a>\<B_u>\<B_x>\<B_i>\<B_l>\<B_i>\<B_a>\<B_r>\<B_y>_\<B_f>\<B_a>\<B_c>\<B_t>\<B_s>"
-      and "auxfacts" = "\<B_a>\<B_u>\<B_x>\<B_i>\<B_l>\<B_i>\<B_a>\<B_r>\<B_y>_\<B_f>\<B_a>\<B_c>\<B_t>\<B_s>"
+  abbrevs "is" = "\<^bold>i\<^bold>s"
+      and "as" = "\<^bold>a\<^bold>s"
+      and "register" = "\<^bold>r\<^bold>e\<^bold>g\<^bold>i\<^bold>s\<^bold>t\<^bold>e\<^bold>r"
+      and "in" = "\<^bold>i\<^bold>n"
+      and "with" = "\<^bold>w\<^bold>i\<^bold>t\<^bold>h"
+      and "auxiliary_facts" = "\<^bold>w\<^bold>i\<^bold>t\<^bold>h \<^bold>f\<^bold>a\<^bold>c\<^bold>t\<^bold>s"
+      and "auxfacts" = "\<^bold>w\<^bold>i\<^bold>t\<^bold>h \<^bold>f\<^bold>a\<^bold>c\<^bold>t\<^bold>s"
+      and "proc" = "\<^bold>p\<^bold>r\<^bold>o\<^bold>c"
+      and "param" = "\<^bold>p\<^bold>a\<^bold>r\<^bold>a\<^bold>m"
+      and ";;" = "\<bbar>"
 begin
 
 text \<open>The fundamental theory for \<nu>-system\<close>
@@ -18,13 +22,45 @@ declare [[quick_and_dirty = true]]
 bundle show_more1 = [[show_hyps = true, show_types = true, show_sorts = true]]
 bundle show_more = [[show_hyps = true, show_types = true]]
 
-named_theorems abst_expn "expansion theorems for abstractions"
+named_theorems \<nu>share
+named_theorems \<nu>equable
+
+subsubsection \<open>Syntax and Notations\<close>
+
+consts "ARBITRARY___" :: 'a ("\<cdots>") \<comment>\<open>merely a sugar for documenting\<close>
+
+definition PropBlock :: "prop \<Rightarrow> prop" ("\<medium_left_bracket> _ \<medium_right_bracket>" [0] 1000) where "PropBlock p \<equiv> p"
+  \<comment>\<open>The block of proposition has specific meaning in \<nu>-system.
+  @{prop "A \<Longrightarrow> B \<Longrightarrow> C"} represents an forward construction rule to finally construct @{term C}.
+  The construction rule could be high-order parametric, e.g. @{prop "A \<Longrightarrow> \<medium_left_bracket> B \<Longrightarrow> C \<Longrightarrow> D \<medium_right_bracket> \<Longrightarrow> E"},
+    and in those cases the high-order parameter is wrapped by @{term Pure.prop} to become an atomic
+    premise in order to disambiguate with the semantics of nested hypothesises.\<close>
+lemmas  PropBlock_I = PropBlock_def[THEN equal_elim_rule2]
+lemmas  PropBlock_D = PropBlock_def[THEN equal_elim_rule1]
+
+syntax
+  "_pretty_and_" :: "logic \<Rightarrow> logic \<Rightarrow> logic"  ("_/ \<^bold>a\<^bold>n\<^bold>d _" [4,3] 3)
+  "_linebreak_" :: "logic \<Rightarrow> logic" ("//\<zero_width_space>_" [3] 3)
+  "_linebreak_collection_" :: "logic \<Rightarrow> logic \<Rightarrow> logic"  ("_//\<invisible_separator>_" [4,3] 3)
+  "_with_" :: "logic \<Rightarrow> logic \<Rightarrow> logic" ("_/ \<^bold>w\<^bold>i\<^bold>t\<^bold>h _" [2,1] 1)
+  (* "_is_" :: "logic \<Rightarrow> logic \<Rightarrow> logic" ("_ \<^bold>i\<^bold>s _" [5,5] 4)
+  "_in_" :: "logic \<Rightarrow> logic \<Rightarrow> logic" ("_ \<^bold>i\<^bold>n _" [5,5] 4)
+  "_as_" :: "logic \<Rightarrow> logic \<Rightarrow> logic" ("_ \<^bold>a\<^bold>s _" [5,5] 4) *)
+translations
+  "a \<^bold>a\<^bold>n\<^bold>d b \<^bold>a\<^bold>n\<^bold>d c" <= "(a \<^bold>a\<^bold>n\<^bold>d b) \<^bold>a\<^bold>n\<^bold>d c"
+  "_linebreak_collection_ a (_linebreak_collection_ b c)" <= "_linebreak_collection_ (_linebreak_collection_ a b) c"
+text \<open> `_pretty_and_` suppresses parentheses in the printing. For example, both the term
+  "1 and 2 and 3" and  "(1 and 2) and 3" are printed identically, as 1 \<^bold>a\<^bold>n\<^bold>d 2 \<^bold>a\<^bold>n\<^bold>d 3". 
+  It is useful to represent a collection of object which has some complicated inner structure
+    (e.g. a binary tree) that is not intended to be displayed to user.\<close>
+
+named_theorems typing_expn "expansion theorems for abstractions"
 
 datatype zint = Gz | Gi int
 text\<open> Type @{typ zint} is used to represent ownership. @{term "Gi i"} represents
   $2^{-i}$ part of the ownership, and @{term "Gi 0"} is the total. @{term Gz} represents
   some ownership of unknown quantity. Any value of @{type zint} represents
-  some part of (or total) ownership. The empty ownership is represented
+  some part (or the total) of ownership. The empty ownership is represented
   by further structure like @{typ "zint option"} as @{term None}\<close>
 
 instantiation zint :: comm_monoid_add begin
@@ -43,29 +79,29 @@ end
 definition K_def[simp]: "K a b = a"
 lemma K_intro[intro]: "(\<forall>x y. f x y = x) \<Longrightarrow> f = K" by (simp add: ext)
 
-section\<open>Fundamentals for low level representation\<close>
+section\<open>Low representation for semantics\<close>
 
-datatype layout = la_i nat | la_p nat | la_s layout
-  | la_a layout nat | la_z | la_C layout layout
+datatype llty = la_i nat | la_p nat | la_s llty
+  | la_a llty nat | la_z | la_C llty llty
 
-class llty = fixes layout :: "'a itself \<Rightarrow> layout"
+class lrep = fixes llty :: "'a itself \<Rightarrow> llty"
   \<comment>\<open>The class for basic low level types\<close>
 
 text \<open>The ability for memory allocation\<close>
-class zero_llty = llty +
+class zero_lrep = lrep +
   fixes lty_zero :: "'a"
 
 text \<open>The ability for equality comparison\<close>
-class ceq_llty = llty +
+class ceq_lrep = lrep +
   fixes ceqable :: "('a * 'a) \<Rightarrow> bool"
   fixes ceq :: "('a * 'a) \<Rightarrow> bool"
   assumes ceqable_sym[ac_simps]: "ceqable (x,y) = ceqable (y,x)"
   assumes ceq_refl[simp]: "ceqable (x,x) \<Longrightarrow> ceq (x,x)"
-  assumes ceq_sym: "ceqable (x,y) \<Longrightarrow> ceq (x,y) \<longleftrightarrow> ceq (y,x)"
+  assumes ceq_sym[ac_simps]: "ceqable (x,y) \<Longrightarrow> ceq (x,y) \<longleftrightarrow> ceq (y,x)"
   assumes ceq_trans: "ceqable (x,y) \<Longrightarrow> ceqable (y,z) \<Longrightarrow> ceqable (x,z)
     \<Longrightarrow> ceq(x,y) \<Longrightarrow> ceq (y,z) \<Longrightarrow> ceq (x,z)"
 
-class sharable_llty = llty + 
+class sharable_lrep = lrep + 
   fixes revert :: "'a * 'a \<Rightarrow> bool"
     and sharable :: "'a \<Rightarrow> bool"
     and share :: "'a \<Rightarrow> zint \<Rightarrow> 'a"
@@ -76,91 +112,265 @@ class sharable_llty = llty +
   assumes share_id[simp]: "share x (Gi 0) = x"
   assumes share_assoc[simp]: "share (share x a) b = share x (a + b)"
 
-class masharable_llty = sharable_llty +
+class naive_lrep = sharable_lrep +
   assumes marsharable_sha[simp]: "sharable x = True"
   assumes marsharable_dp[simp]: "dpriv = id"
   assumes marsharable_sh[simp]: "share = K"
   assumes marsharable_rt[simp]: "revert xy = True"  
 
-datatype 'a state = StatOn 'a | STrap | SNeg
+datatype ('a,'b) nu = Nu "('a::lrep) * 'b \<Rightarrow> bool"
 
-datatype ('a,'b) nu = Nu "('a::llty) * 'b \<Rightarrow> bool"
-definition abstraction :: "('a::llty) \<Rightarrow> ('a,'b) nu \<Rightarrow> 'b \<Rightarrow> bool" ("(_/ \<nuLinkL> _ \<nuLinkR>/ _)" [15,15,15] 14)
-  where abstraction_def: "abstraction p N x = (case N of Nu R \<Rightarrow> R (p,x))"
+definition NuTyp :: "'b \<Rightarrow> ('a::lrep,'b) nu \<Rightarrow> 'a set" (infix "\<tycolon>" 15) \<comment>\<open>shortcut keys ":ty:"\<close>
+  where "(x \<tycolon> N) = {p. case N of Nu R \<Rightarrow> R (p,x) }"
+abbreviation NuTyping :: "('a::lrep) \<Rightarrow> ('a,'b) nu \<Rightarrow> 'b \<Rightarrow> bool" ("(_/ \<nuLinkL> _ \<nuLinkR>/ _)" [27,15,27] 26) \<comment>\<open>shortcut keys "--<" and ">--"\<close>
+  where  "(p \<nuLinkL> N \<nuLinkR> x) \<equiv> p \<in> (x \<tycolon> N)"
+definition Inhabited :: " 'a set \<Rightarrow> bool" where "Inhabited s \<equiv> (\<exists>x. x \<in> s)"
+abbreviation InhabitTyp :: " 'b \<Rightarrow> ('a::lrep,'b) nu \<Rightarrow> bool" (infix "\<ratio>" 15)  \<comment>\<open>shortcut keys ":TY:"\<close>
+  where  "(x \<ratio> N) \<equiv> Inhabited (x \<tycolon> N)"
+text \<open>The @{term "x \<tycolon> N"} is a predication specifying concrete values,
+  e.g. @{prop "a_concrete_int32 \<in> ((42::nat) \<tycolon> N 32) "} and also @{prop "state \<in> State ((42 \<tycolon> N) \<times> (24 \<tycolon> N) \<times> \<cdots> )"}.
+  It constitutes basic elements in specification.
+  The @{prop "p \<nuLinkL> N \<nuLinkR> x"} as the abbreviation of $p \<in> (x \<tycolon> N)$ is an abstraction between concrete value @{term p} and
+  abstracted {\it image} @{term x} via the \<nu>-{\it abstractor} @{term N} which defines the abstraction relationship itself.
+  The next @{prop "x \<ratio> N"} is a proposition stating @{term x} is an image of abstractor @{term N} and therefore
+  the \<nu>-type @{term "x \<tycolon> N"} is inhabited. Basically it is used to derive implicated conditions of images,
+  e.g. @{prop "(42 \<ratio> N 32) \<Longrightarrow> 42 < 2^32"}\<close>
 
-definition Nu_SE :: "('a::llty,'b) nu \<Rightarrow> 'b \<Rightarrow> bool" where
-  Nu_SE_def:  "Nu_SE N x \<longleftrightarrow> (\<exists>p. p \<nuLinkL> N \<nuLinkR> x)"
-definition NuPred :: "('a::llty,'b) nu \<Rightarrow> 'b \<Rightarrow> 'a set" (infix "\<nuPred>" 72) where
-  NuPred_def: "NuPred N x = {p. (p \<nuLinkL> N \<nuLinkR> x) }"
+lemma [simp]: "p \<nuLinkL> Nu R \<nuLinkR> x \<equiv> R (p,x)" unfolding NuTyp_def by simp
+lemma inhabited[dest]: "p \<nuLinkL> N \<nuLinkR> x \<Longrightarrow> x \<ratio> N" unfolding Inhabited_def by auto
+lemma [elim]: "Inhabited (U \<times> V) \<Longrightarrow> (Inhabited U \<Longrightarrow> Inhabited V \<Longrightarrow> PROP C) \<Longrightarrow> PROP C" unfolding Inhabited_def by auto
 
-lemma abstraction_SE: "p \<nuLinkL> N \<nuLinkR> x \<Longrightarrow> Nu_SE N x" by (auto simp add: Nu_SE_def)
+definition Nu_Share :: "('a::sharable_lrep,'b) nu \<Rightarrow> ('b \<Rightarrow> zint \<Rightarrow> 'b) \<Rightarrow> bool"
+  where  "Nu_Share N f \<longleftrightarrow> (\<forall>z p x. (p \<nuLinkL> N \<nuLinkR> x) \<longrightarrow> (share p z \<nuLinkL> N \<nuLinkR> f x z))"
+lemma \<nu>share_masharable[\<nu>share]: "Nu_Share N K" for N :: "('a::naive_lrep, 'b) nu" unfolding Nu_Share_def by simp
+definition \<nu>Equalable :: "('a::ceq_lrep, 'b) nu \<Rightarrow> ('b \<times> 'b \<Rightarrow> bool) \<Rightarrow> bool"
+  where "\<nu>Equalable N f \<longleftrightarrow> (\<forall>p1 p2 x1 x2. (p1 \<nuLinkL> N \<nuLinkR> x1) \<and> (p2 \<nuLinkL> N \<nuLinkR> x2) \<longrightarrow> ceqable (p1,p2) = f (x1,x2))"
 
-definition Nu_Share :: "('a::sharable_llty,'b) nu \<Rightarrow> ('b \<Rightarrow> zint \<Rightarrow> 'b) \<Rightarrow> bool" where
-  Nu_Share_def: "Nu_Share N f \<longleftrightarrow> (\<forall>z p x. (p \<nuLinkL> N \<nuLinkR> x) \<longrightarrow> (share p z \<nuLinkL> N \<nuLinkR> f x z))"
+lemma K_rew: "(\<lambda>x. c) =  (K c)" by auto
+lemma [simp]: "\<nu>Equalable N (\<lambda>x. c) = \<nu>Equalable N (K c)" by (auto simp add: K_rew)
+lemma [simp]: "Nu_Share N (\<lambda>x z. x) = Nu_Share N K" by (auto simp add: K_rew)
 
 section\<open>Structures for construction\<close>
 
-definition instr_comp (infixl "\<diamondop>" 55) where  "instr_comp = (o)"
-text \<open> The operator @{term instr_comp} as an alias for the functional composition operator
-   is defined  for the specific purpose for instruction composition in \<nu>-system.  \<close>
+subsubsection \<open>Auxiliary name tag\<close>
 
-type_synonym label = ind
-datatype 'a register = Register label 'a
+datatype name_tag = NAME_TAG "unit \<Rightarrow> unit"
+datatype name2_tag = NAME2_TAG "unit \<Rightarrow> unit \<Rightarrow> unit"
+lemma [cong]: "NAME_TAG x \<equiv> NAME_TAG x" and [cong]: "NAME2_TAG y \<equiv> NAME2_TAG y" using reflexive .
+syntax "_NAME_" :: "idt \<Rightarrow> name_tag" ("NAME _" [0] 1000)
+  "_NAME2_" :: "idt => idt => name_tag" ("NAME2 _ _" [0,0] 1000)
+translations "NAME name" == "CONST NAME_TAG (\<lambda>name. ())"
+  "NAME2 name1 name2" == "CONST NAME2_TAG (\<lambda>name1 name2. ())"
+
+definition Named :: "name_tag \<Rightarrow> 'a \<Rightarrow> 'a" where "Named name x = x" \<comment>\<open>name tag\<close>
+syntax "_named_" :: "logic \<Rightarrow> idt \<Rightarrow> logic" (infix "named" 4)
+translations "x named name" == "CONST Named (NAME name) x"
+ML_val \<open> Syntax.read_term @{context} "AAA named yy" \<close>
+
+subsubsection \<open>Register and its collection\<close>
+
+datatype void = void \<comment>\<open> End of the stack \<close>
+definition Void :: "void set" where "Void = {void}" 
+text \<open>The name `void` coincides that, when a procedure has no input arguments,
+  the \<nu>-type for the input would exactly be @{term Void}. \<close>
+lemma [simp,intro]: "void \<in> Void" unfolding VoidTy_def by simp
+translations "a" <= "a \<^bold>a\<^bold>n\<^bold>d CONST Void"
+
+datatype 'a register = Register name_tag 'a
   \<comment>\<open> Register label value
     where `label` is a free variable representing name of the register by its variable name\<close>
-notation Register ("\<B_r>\<B_e>\<B_g>\<B_i>\<B_s>\<B_t>\<B_e>\<B_r> _ \<B_i>\<B_s> _" [4,4] 3)
+syntax "_register_as_" :: "idt \<Rightarrow> 'a \<Rightarrow> 'a register" ("\<^bold>r\<^bold>e\<^bold>g\<^bold>i\<^bold>s\<^bold>t\<^bold>e\<^bold>r _ \<^bold>a\<^bold>s _" [5,5] 4)
+translations "_register_as_ name exp" == "CONST Register (NAME name) exp"
+term "Register (NAME a) b"
 
-definition RegisterSet :: "ind \<Rightarrow> 'a set \<Rightarrow> 'a register set" where
-  RegisterSet_def: "RegisterSet name s = {r. case r of Register name' x \<Rightarrow> name' = name \<and> x \<in> s}"
-notation RegisterSet ("_ \<B_n>\<B_a>\<B_m>\<B_e>\<B_d> _" [4,4] 3)
-   and RegisterSet ("\<B_r>\<B_e>\<B_g>\<B_i>\<B_s>\<B_t>\<B_e>\<B_r> _ \<B_i>\<B_n> _" [4,4] 3)
+definition RegisterTy :: "name_tag \<Rightarrow> 'a set \<Rightarrow> 'a register set" where
+  RegisterTy_def: "RegisterTy name s = {r. case r of Register name' x \<Rightarrow> name' = name \<and> x \<in> s}"
+syntax "_register_set_" :: "idt \<Rightarrow> 'a set \<Rightarrow> 'a register set" ("\<^bold>r\<^bold>e\<^bold>g\<^bold>i\<^bold>s\<^bold>t\<^bold>e\<^bold>r _ \<^bold>i\<^bold>n _" [5,5] 4)
+translations "_register_set_ name S" == "CONST RegisterTy (NAME name) S"
+lemma [simp]: "Register v x \<in> RegisterTy v' T \<longleftrightarrow> v = v' \<and> x \<in> T" unfolding RegisterTy_def by  simp
 
-definition PrettyAnd :: " 'a \<Rightarrow> 'b \<Rightarrow> 'a \<times> 'b " (infixr "and'_pair" 5)  where
-  PrettyAnd_def: "(PrettyAnd) = Pair"
-definition PrettyAndSet :: " 'a set \<Rightarrow> 'b set \<Rightarrow> ('a \<times> 'b) set " (infixr "and'_set" 5)  where
-  PrettyAndSet_def: "(PrettyAndSet) = (\<times>)"
-text \<open> `PrettyAnd` and `PrettyAndSet` are two alias for pairing operator and
-  production set operator respectively, with special pretty printing settings to
-  prevent parentheses in the printing. For example, both the term
-  @{term "1 and_pair 2 and_pair 3"} and @{term "(1 and_pair 2) and_pair 3"}
-  are printed identically, as "1 \<B_a>\<B_n>\<B_d> 2 \<B_a>\<B_n>\<B_d> 3". 
-  It is useful to represent a collection of object which has some complicated inner structure
-    (e.g. a binary tree) that is not intended to be displayed to user.\<close>
-syntax "\<B_a>\<B_n>\<B_d>" :: "logic \<Rightarrow> logic \<Rightarrow> logic"  ("_/ \<B_a>\<B_n>\<B_d> _" [6,5] 5)
+definition And :: " 'a \<Rightarrow> 'b \<Rightarrow> 'a \<times> 'b " (infixr "and'_pair" 3)  where "And = Pair"
+definition AndTy :: " 'a set \<Rightarrow> 'b set \<Rightarrow> ('a \<times> 'b) set " (infixr "and'_ty" 3)  where  "AndTy = (\<times>)"
 translations
-  "a \<B_a>\<B_n>\<B_d> b" <= "a and_pair b"
-  "a \<B_a>\<B_n>\<B_d> b" <= "a and_set b"
-  "a \<B_a>\<B_n>\<B_d> b \<B_a>\<B_n>\<B_d> c" <= "((a \<B_a>\<B_n>\<B_d> b) \<B_a>\<B_n>\<B_d> c)"
+  "a \<^bold>a\<^bold>n\<^bold>d b" <= "a and_pair b"
+  "a \<^bold>a\<^bold>n\<^bold>d b" <= "a and_ty b"
+lemma [simp]: "(a and_pair b) \<in> (A and_ty B) \<longleftrightarrow> a \<in> A \<and> b \<in> B" unfolding AndTy_def And_def by simp
 
-class register_collection = llty
-  \<comment> \<open> A register_collection is always a llty, but NOT vice versa.
-    register_collection ::= unit | register | register_collection \<times> register_collection.
-    Also note register_collection is a binary tree.\<close>
+class register_collection = lrep
+  \<comment> \<open> A register_collection is always a lrep, but a lrep may not a register collection.
+    register_collection ::= void | register | register_collection \<times> register_collection.
+    Also note register_collection is a binary tree, not only a register list.\<close>
 
-datatype ('a, 'r) with_registers = WithRegisters 'a 'r (infix "with'_registers" 4)
-type_notation with_registers ("_/ with _" [5,5] 4)
-definition WithRegistersSet :: " 'a set \<Rightarrow> 'b set \<Rightarrow> ('a with 'b) set" (infix "with'_set" 4) where
-  WithRegistersSet_def: "WithRegistersSet s t = {x. case x of WithRegisters a b \<Rightarrow> a \<in>s \<and> b \<in> t}"
-syntax "\<B_w>\<B_i>\<B_t>\<B_h>" :: "logic \<Rightarrow> logic \<Rightarrow> logic" ("_/ \<B_w>\<B_i>\<B_t>\<B_h> _" [5,5] 4)
-translations
-  "a \<B_w>\<B_i>\<B_t>\<B_h> b" <= "a with_registers b"
-  "a \<B_w>\<B_i>\<B_t>\<B_h> b" <= "a with_set b"
+instantiation void :: register_collection begin
+definition llty_void :: "void itself \<Rightarrow> llty" where [simp]: "llty_void _ = la_z"
+instance by standard
+end
 
-definition CodeBlock :: " 'a state \<Rightarrow> 'a state \<Rightarrow> bool" where
-  CodeBlock_def: "CodeBlock var exp \<longleftrightarrow> (var = exp) \<and> (var \<noteq> STrap) "
+instantiation register :: (lrep) register_collection begin
+definition register_unit :: "'a register itself \<Rightarrow> llty" where [simp]: "register_unit _ = la_z"
+instance by standard
+end
 
-definition SpecTop :: "prop \<Rightarrow> prop \<Rightarrow> prop" where
-  SpecTop_def: "SpecTop \<equiv> (&&&)"
+instantiation prod :: (lrep,lrep) lrep begin
+definition llty_prod :: "('a \<times> 'b) itself \<Rightarrow> llty" where [simp]: "llty_prod _ = la_C (llty TYPE('a)) (llty TYPE('b))"
+instance by standard
+end
+
+instantiation prod :: (register_collection,register_collection) register_collection begin instance by standard end
+
+subsubsection \<open>The \<nu>-system VM and Procedure construction structures\<close>
+
+definition Stack_Delimiter (infixr "\<bbar>" 13) where [simp]:"Stack_Delimiter = (\<times>)"
+definition End_of_Contextual_Stack :: " 'a \<Rightarrow> 'a " where "End_of_Contextual_Stack x = x" \<comment> \<open>A tag for printing sugar\<close>
+translations "a" <= "a \<bbar> CONST End_of_Contextual_Stack x" \<comment> \<open>hide the end\<close>
+lemma [simp]: "(a,b) \<in> A \<bbar> B \<longleftrightarrow> a \<in> A \<and> b \<in> B" unfolding Stack_Delimiter_def by simp
+
+text \<open>The procedure construction context.\<close>
+datatype ('a, 'r) "proc_ctx"  = Proc_Ctx 'a 'r
+declare proc_ctx.split[split]
+type_notation "proc_ctx" ("_/ \<flower> _" [2,2] 1)
+definition Proc_CtxTy :: " ('a::lrep) set \<Rightarrow> ('b::register_collection) set \<Rightarrow> ('a \<flower> 'b) set" (infix "\<flower>" 4)
+  where "Proc_CtxTy s t = {x. case x of Proc_Ctx a b \<Rightarrow> a \<in>s \<and> b \<in> t}"
+syntax "_no_registers_" :: logic ("\<^bold>n\<^bold>o \<^bold>r\<^bold>e\<^bold>g\<^bold>i\<^bold>s\<^bold>t\<^bold>e\<^bold>r\<^bold>s")
+   "_empty_stack_" :: logic ("\<^bold>e\<^bold>m\<^bold>p\<^bold>t\<^bold>y \<^bold>s\<^bold>t\<^bold>a\<^bold>c\<^bold>k")
+translations "x \<flower> \<^bold>n\<^bold>o \<^bold>r\<^bold>e\<^bold>g\<^bold>i\<^bold>s\<^bold>t\<^bold>e\<^bold>r\<^bold>s" == "x \<flower> CONST Void"
+  "\<^bold>e\<^bold>m\<^bold>p\<^bold>t\<^bold>y \<^bold>s\<^bold>t\<^bold>a\<^bold>c\<^bold>k \<flower> x" <= "CONST End_of_Contextual_Stack s \<flower> x"
+term "A \<bbar> B \<bbar> End_of_Contextual_Stack R \<flower> Void"
+lemma [simp]: "(Proc_Ctx s r) \<in> (T \<flower> U) \<equiv> s \<in> T \<and> r \<in> U" by (simp add: Proc_CtxTy_def)
+lemma Proc_CtxTy_elim[elim]: "c \<in> (T \<flower> U) \<Longrightarrow> (\<And>s r. c = (Proc_Ctx s r) \<Longrightarrow> s \<in> T \<Longrightarrow> r \<in> U \<Longrightarrow> C) \<Longrightarrow> C" by (cases c) auto
+lemma [dest]: "Proc_Ctx s r \<in> (T \<flower> U) \<Longrightarrow> s \<in> T" and [dest]: "Proc_Ctx s r \<in> (T \<flower> U) \<Longrightarrow> r \<in> U" by simp+
+lemma Proc_CtxTy_intro[intro]: "s \<in> T \<Longrightarrow> r \<in> U \<Longrightarrow> Proc_Ctx s r \<in> (T \<flower> U)" by (simp add: Proc_CtxTy_def)
+
+
+datatype 'a state = StatOn 'a | STrap | SNeg
+text\<open> The basic state of the \<nu>-system virtual machine is represented by type @{typ "'a state"}.
+  The valid state @{term "StatOn p"} essentially has two major form, one without registers and another one with them,
+      \<^item> @{term "StatOn (x1, x2, \<cdots>, xn, void)"},
+      \<^item> @{term "StatOn (Proc_Ctx (x1, x2, \<cdots>, xn, void ) (\<^bold>r\<^bold>e\<^bold>g\<^bold>i\<^bold>s\<^bold>t\<^bold>e\<^bold>r r1 \<^bold>a\<^bold>s y1 and_pair \<^bold>r\<^bold>e\<^bold>g\<^bold>i\<^bold>s\<^bold>t\<^bold>e\<^bold>r r2 \<^bold>a\<^bold>s y2 and_pair \<cdots>))"},
+  where @{term "(x1, x2, \<cdots>, xn, void)"} represents the stack in the state, with @{term x\<^sub>i} as the i\<^sup>t\<^sup>h element on the stack.
+  The @{term STrap} is trapped state due to invalid operations like zero division.
+  The negative state @{term SNeg} represents the admissible error situation that is not considered in partial correctness.
+  For example, @{term SNeg} may represents an admissible crash, and in that case the partial correctness certifies that
+    ``if the program exits normally, the output would be correct''.\<close>
+declare state.split[split]
+definition StrictStateTy :: " 'a set \<Rightarrow> 'a state set" ("\<S_S> _" [56] 55)
+  where "\<S_S> T = {s. case s of StatOn x \<Rightarrow> x \<in> T | STrap \<Rightarrow> False | SNeg \<Rightarrow> False}"
+definition LooseStateTy :: " 'a set \<Rightarrow> 'a state set" ("\<S> _" [56] 55)
+  where "\<S> T = {s. case s of StatOn x \<Rightarrow> x \<in> T | STrap \<Rightarrow> False | SNeg \<Rightarrow> True}"
+lemma [simp]: "StatOn x \<in> \<S_S> T \<equiv> x \<in> T" and [simp]: "\<not> (SNeg \<in> \<S_S> T)" and [simp]: "\<not> (STrap \<in> \<S_S> T)"
+  and [simp]: "StatOn x \<in> \<S> T \<equiv> x \<in> T" and [simp]: "SNeg \<in> \<S> T" and [simp]: "\<not> (STrap \<in> \<S> T)"
+  by (simp_all add: StrictStateTy_def LooseStateTy_def)
+lemma [dest]: "s \<in> \<S_S> T \<Longrightarrow> Inhabited T" unfolding Inhabited_def by (cases s) auto
+    \<comment>\<open>The inhabited property can be inferred from @{term StrictStateTy} only rather than @{term LooseStateTy}. \<close>
+lemma StrictStateTy_elim: "s \<in> \<S_S> T \<Longrightarrow> (\<And>x. s = StatOn x \<Longrightarrow> x \<in> T \<Longrightarrow> C) \<Longrightarrow> C" by (cases s) auto
+lemma LooseStateTy_elim: "s \<in> \<S> T \<Longrightarrow> (\<And>x. s = StatOn x \<Longrightarrow> x \<in> T \<Longrightarrow> C) \<Longrightarrow> (s = SNeg \<Longrightarrow> C) \<Longrightarrow> C" by (cases s) auto
+lemma LooseStateTy_upgrade: "s \<in> \<S> T \<Longrightarrow> s \<noteq> SNeg \<Longrightarrow> s \<in> \<S_S> T" by (cases s) auto
+lemma StrictStateTy_degrade: "s \<in> \<S_S> T \<Longrightarrow> s \<in> \<S> T" by (cases s) auto
+lemma LooseStateTy_introByStrict: "(s \<noteq> SNeg \<Longrightarrow> s \<in> \<S_S> T) \<Longrightarrow> s \<in> \<S> T" by (cases s) auto
+
+definition ExTyp :: "('a \<Rightarrow> 'b set) \<Rightarrow> 'b set" (binder "\<exists>* " 10) where "ExTyp T = {x. (\<exists>z. x \<in> T z)}"
+lemma [simp]: "x \<in> ExTyp T \<equiv> (\<exists>z. x \<in> T z)" unfolding ExTyp_def by auto
+lemma [simp]: "\<S_S> (ExTyp T) = (\<exists>* x. \<S_S> (T x))" unfolding ExTyp_def
+proof auto
+  fix x z show "x \<in> \<S_S> {x. \<exists>z. x \<in> T z} \<Longrightarrow> \<exists>z. x \<in> \<S_S> T z" and "x \<in> \<S_S> T z \<Longrightarrow> x \<in> \<S_S> {x. \<exists>z. x \<in> T z}" by (cases x; auto)+
+qed
+lemma [simp]: "\<S> (ExTyp T) = (\<exists>* x. \<S> (T x))" unfolding ExTyp_def
+proof auto
+  fix x z show "x \<in> \<S> {x. \<exists>z. x \<in> T z} \<Longrightarrow> \<exists>z. x \<in> \<S> T z " and "x \<in> \<S> T z \<Longrightarrow> x \<in> \<S> {x. \<exists>z. x \<in> T z}" by (cases x; auto)+
+qed
+
+abbreviation Procedure :: "('a \<Rightarrow> 'b state) \<Rightarrow> 'a set \<Rightarrow> 'b set \<Rightarrow> bool" ("\<^bold>p\<^bold>r\<^bold>o\<^bold>c _ \<llangle> _ \<longmapsto> _ \<rrangle>" [4,2,2] 5)
+  where "Procedure f T U \<equiv> (\<forall>a. a \<in> T \<longrightarrow> f a \<in> \<S> U)"
+
+definition bind :: " 'a state \<Rightarrow> ('a \<Rightarrow> 'b state) \<Rightarrow> 'b state " \<comment>\<open>monadic bind\<close>
+  where "bind s f = (case s of StatOn x \<Rightarrow> f x | STrap \<Rightarrow> STrap | SNeg \<Rightarrow> SNeg)"
+definition instr_comp :: "('a \<Rightarrow> 'b state) \<Rightarrow> ('b \<Rightarrow> 'c state) \<Rightarrow> 'a \<Rightarrow> 'c state"  (infixr "\<nuInstrComp>" 75) 
+  where "instr_comp f g s = bind (f s) g" \<comment>\<open>It is NOT monadic `then` operator (\<then>)!\<close>
+definition nop :: " 'a \<Rightarrow> 'a state" where "nop = StatOn" \<comment>\<open>the instruction `no-operation`\<close>
+definition call :: "('a \<Rightarrow> 'b state) \<Rightarrow> ('a \<flower> 'r) \<Rightarrow> ('b \<flower> 'r) state"
+  where "call f s = (case s of Proc_Ctx x r \<Rightarrow> bind (f x) (\<lambda>x. StatOn (Proc_Ctx x r)))"
+definition begin_proc_ctx :: " 'a \<Rightarrow> ('a \<flower> void) state" where "begin_proc_ctx x = StatOn (Proc_Ctx x void)"
+definition end_proc_ctx :: " 'a \<flower> 'b \<Rightarrow> 'a state" where "end_proc_ctx ctx = (case ctx of Proc_Ctx x y \<Rightarrow> StatOn x)"
+
+lemma nop: "\<^bold>p\<^bold>r\<^bold>o\<^bold>c nop \<llangle> T \<longmapsto> T \<rrangle>" unfolding nop_def by auto
+lemma call: "\<^bold>p\<^bold>r\<^bold>o\<^bold>c f \<llangle> U \<longmapsto> V \<rrangle> \<Longrightarrow> \<^bold>p\<^bold>r\<^bold>o\<^bold>c call f \<llangle> U \<flower> W \<longmapsto> V \<flower> W \<rrangle>"
+  unfolding call_def by  (auto simp add: bind_def)
+lemma end_proc_ctx: "\<^bold>p\<^bold>r\<^bold>o\<^bold>c end_proc_ctx \<llangle> T \<flower> R \<longmapsto> T \<rrangle>" unfolding end_proc_ctx_def by auto
+
+subsection \<open>Top-level constructions and rules\<close>
+
+definition CurrentConstruction :: " 'a state \<Rightarrow> 'a set \<Rightarrow> bool " ("\<^bold>c\<^bold>u\<^bold>r\<^bold>r\<^bold>e\<^bold>n\<^bold>t _ \<B_r>\<B_e>\<^bold>s\<B_u>\<B_l>\<B_t>\<^bold>s \<^bold>i\<^bold>n/ _" [1000,5] 0)
+  where "CurrentConstruction s S \<longleftrightarrow> s \<in> \<S_S> S"
+definition PendingConstruction :: " ('a \<Rightarrow> 'b state) \<Rightarrow> 'a state \<Rightarrow> 'b set \<Rightarrow> bool " ("\<B_p>\<B_e>\<B_n>\<B_d>\<^bold>i\<^bold>n\<B_g> _ \<^bold>o\<^bold>n _ \<B_r>\<B_e>\<^bold>s\<B_u>\<B_l>\<B_t>\<^bold>s \<^bold>i\<^bold>n/ _" [1000,1000,1] 0)
+  where "PendingConstruction f s S \<longleftrightarrow> bind s f \<in> \<S> S"
+
+definition CodeBlock :: " 'a state \<Rightarrow> 'b => 'b set \<Rightarrow> ('b \<Rightarrow> 'a state) \<Rightarrow> bool" where
+  CodeBlock_def: "CodeBlock stat arg ty prog \<longleftrightarrow> (arg \<in> ty \<and> prog arg = stat \<and> stat \<noteq> SNeg)"
+syntax "_codeblock_exp_" :: "idt \<Rightarrow> logic \<Rightarrow> logic \<Rightarrow> bool"  ("\<^bold>c\<^bold>o\<^bold>d\<^bold>e\<^bold>b\<^bold>l\<^bold>o\<^bold>c\<^bold>k _  \<^bold>a\<^bold>s '\<open>_'\<close> \<^bold>f\<^bold>o\<^bold>r \<^bold>a\<B_r>\<B_g>\<B_u>\<B_m>\<B_e>\<B_n>\<B_t>\<^bold>s '\<open>_'\<close> " [100,0,0] 3)
+syntax "_codeblock_" :: "idt \<Rightarrow> logic \<Rightarrow> bool" ("\<^bold>c\<^bold>o\<^bold>d\<^bold>e\<^bold>b\<^bold>l\<^bold>o\<^bold>c\<^bold>k _ \<^bold>f\<^bold>o\<^bold>r \<^bold>a\<B_r>\<B_g>\<B_u>\<B_m>\<B_e>\<B_n>\<B_t>\<^bold>s '\<open>_'\<close>" [100,0] 3)
+translations "_codeblock_ v ty" <= "CONST CodeBlock v arg ty exp"
+(* translations "_codeblock_exp_ v exp ty" <= "CONST CodeBlock v arg ty exp" *)
+
+definition Fact :: "ind \<Rightarrow> bool \<Rightarrow> prop" ("\<^item> _ : _" [5,0] 4) where Fact_def:"Fact label P \<equiv>Trueprop P"
+
+term "PROP (Fact a b) &&& PROP (Fact c d)"
+definition NoFact :: "prop" ("\<B_n>\<B_o>\<B_t>\<B_h>\<^bold>i\<^bold>n\<B_g>") where "NoFact \<equiv> Trueprop True"
+definition AndFact :: "prop \<Rightarrow> prop \<Rightarrow> prop" (infixr "and'_fact" 3) where AndFact_def:"AndFact \<equiv> (&&&)"
+translations "_linebreak_collection_ P Q" <= "CONST AndFact P Q"
+lemma NoFact: "PROP NoFact" unfolding NoFact_def by fast
+
+definition SpecTop :: "prop \<Rightarrow> prop \<Rightarrow> prop" where SpecTop_def: "SpecTop \<equiv> (&&&)"
 \<comment>\<open> SpecTop focus lemmata
   where the focus is the focused one or multiple HOL propositions intended to be constructed
     the lemmata are several propositions served as auxiliary facts, e.g. post conditions.\<close>
-notation SpecTop ("_/ \<B_a>\<B_u>\<B_x>\<B_i>\<B_l>\<B_i>\<B_a>\<B_r>\<B_y>'_\<B_f>\<B_a>\<B_c>\<B_t>\<B_s>: _ " [1,1] 0)
-lemma Specification_focus: "(P \<B_a>\<B_u>\<B_x>\<B_i>\<B_l>\<B_i>\<B_a>\<B_r>\<B_y>_\<B_f>\<B_a>\<B_c>\<B_t>\<B_s>: Q) \<Longrightarrow> P" unfolding SpecTop_def by (rule conjunctionD1)
-lemma Specification_aux: "(P \<B_a>\<B_u>\<B_x>\<B_i>\<B_l>\<B_i>\<B_a>\<B_r>\<B_y>_\<B_f>\<B_a>\<B_c>\<B_t>\<B_s>: Q) \<Longrightarrow> Q" unfolding SpecTop_def by (rule conjunctionD2)
-lemma Specification_rule_focus: "(P \<B_a>\<B_u>\<B_x>\<B_i>\<B_l>\<B_i>\<B_a>\<B_r>\<B_y>_\<B_f>\<B_a>\<B_c>\<B_t>\<B_s>: Q) \<Longrightarrow> (Q \<Longrightarrow> P \<Longrightarrow> P') \<Longrightarrow> (P' \<B_a>\<B_u>\<B_x>\<B_i>\<B_l>\<B_i>\<B_a>\<B_r>\<B_y>_\<B_f>\<B_a>\<B_c>\<B_t>\<B_s>: Q)"
+notation SpecTop ("SPEC'_TOP _ _")
+  and SpecTop ("_/ \<^bold>w\<^bold>i\<^bold>t\<^bold>h \<^bold>f\<^bold>a\<^bold>c\<^bold>t\<^bold>s:/ _ " [1,1] 0)
+lemma SpecTop_focus[dest]: "(PROP P \<^bold>w\<^bold>i\<^bold>t\<^bold>h \<^bold>f\<^bold>a\<^bold>c\<^bold>t\<^bold>s: PROP Q) \<Longrightarrow> PROP P" unfolding SpecTop_def conjunction_imp .
+lemma SpecTop_facts[dest]: "(PROP P \<^bold>w\<^bold>i\<^bold>t\<^bold>h \<^bold>f\<^bold>a\<^bold>c\<^bold>t\<^bold>s: PROP Q) \<Longrightarrow> PROP Q" unfolding SpecTop_def conjunction_imp .
+lemma SpecTop_imp: "(PROP SpecTop (PROP P) (PROP L) \<Longrightarrow> PROP C) \<equiv> (PROP P \<Longrightarrow> PROP L \<Longrightarrow> PROP C)"
+  unfolding SpecTop_def conjunction_imp .
+lemma SpecTop_I: "PROP P \<Longrightarrow> PROP L \<Longrightarrow> PROP SpecTop (PROP P) (PROP L)" unfolding SpecTop_def using conjunctionI .
+(* lemma Specification_rule_focus: "(P \<^bold>w\<^bold>i\<^bold>t\<^bold>h \<^bold>f\<^bold>a\<^bold>c\<^bold>t\<^bold>s: PROP Q) \<Longrightarrow> (PROP Q \<Longrightarrow> P \<Longrightarrow> P') \<Longrightarrow> (P' \<^bold>w\<^bold>i\<^bold>t\<^bold>h \<^bold>f\<^bold>a\<^bold>c\<^bold>t\<^bold>s: PROP Q)"
     unfolding SpecTop_def by presburger
-lemma Specification_rule_aux: "(P \<B_a>\<B_u>\<B_x>\<B_i>\<B_l>\<B_i>\<B_a>\<B_r>\<B_y>_\<B_f>\<B_a>\<B_c>\<B_t>\<B_s>: Q) \<Longrightarrow> (Q \<Longrightarrow> Q') \<Longrightarrow> (P \<B_a>\<B_u>\<B_x>\<B_i>\<B_l>\<B_i>\<B_a>\<B_r>\<B_y>_\<B_f>\<B_a>\<B_c>\<B_t>\<B_s>: Q')"
-    unfolding SpecTop_def  by presburger
+lemma Specification_rule_aux: "(P \<^bold>w\<^bold>i\<^bold>t\<^bold>h \<^bold>f\<^bold>a\<^bold>c\<^bold>t\<^bold>s: Q) \<Longrightarrow> (Q \<Longrightarrow> Q') \<Longrightarrow> (P \<^bold>w\<^bold>i\<^bold>t\<^bold>h \<^bold>f\<^bold>a\<^bold>c\<^bold>t\<^bold>s: Q')"
+    unfolding SpecTop_def  by presburger *)
+
+theorem apply_proc: "(\<^bold>c\<^bold>u\<^bold>r\<^bold>r\<^bold>e\<^bold>n\<^bold>t s \<B_r>\<B_e>\<^bold>s\<B_u>\<B_l>\<B_t>\<^bold>s \<^bold>i\<^bold>n S \<^bold>w\<^bold>i\<^bold>t\<^bold>h \<^bold>f\<^bold>a\<^bold>c\<^bold>t\<^bold>s: PROP L ) \<Longrightarrow> \<^bold>p\<^bold>r\<^bold>o\<^bold>c f \<llangle> S \<longmapsto> T \<rrangle> \<Longrightarrow>
+  (\<B_p>\<B_e>\<B_n>\<B_d>\<^bold>i\<^bold>n\<B_g> f \<^bold>o\<^bold>n s \<B_r>\<B_e>\<^bold>s\<B_u>\<B_l>\<B_t>\<^bold>s \<^bold>i\<^bold>n T \<^bold>w\<^bold>i\<^bold>t\<^bold>h \<^bold>f\<^bold>a\<^bold>c\<^bold>t\<^bold>s: PROP L )"
+  unfolding CurrentConstruction_def PendingConstruction_def bind_def SpecTop_imp by (rule SpecTop_I) auto
+
+theorem  accept_proc: "\<medium_left_bracket> \<And>s. CodeBlock s a S f \<Longrightarrow> (\<B_p>\<B_e>\<B_n>\<B_d>\<^bold>i\<^bold>n\<B_g> g \<^bold>o\<^bold>n s \<B_r>\<B_e>\<^bold>s\<B_u>\<B_l>\<B_t>\<^bold>s \<^bold>i\<^bold>n T \<^bold>w\<^bold>i\<^bold>t\<^bold>h \<^bold>f\<^bold>a\<^bold>c\<^bold>t\<^bold>s: PROP L ) \<medium_right_bracket> \<Longrightarrow>
+  CodeBlock s' a S (f \<nuInstrComp> g) \<Longrightarrow> (\<^bold>c\<^bold>u\<^bold>r\<^bold>r\<^bold>e\<^bold>n\<^bold>t s' \<B_r>\<B_e>\<^bold>s\<B_u>\<B_l>\<B_t>\<^bold>s \<^bold>i\<^bold>n T \<^bold>w\<^bold>i\<^bold>t\<^bold>h \<^bold>f\<^bold>a\<^bold>c\<^bold>t\<^bold>s: (PROP L))" for L :: "prop"
+  unfolding PropBlock_def CodeBlock_def instr_comp_def CurrentConstruction_def PendingConstruction_def
+proof (rule SpecTop_I)
+  assume a: "(\<And>s. a \<in> S \<and> f a = s \<and> s \<noteq> SNeg \<Longrightarrow> SPEC_TOP (bind s g \<in> \<S> T) (PROP L))" and b: " a \<in> S \<and> bind (f a) g = s' \<and> s' \<noteq> SNeg"
+  from b have sa: "a \<in> S \<and> f a = f a \<and> f a \<noteq> SNeg" by (cases "f a") (auto simp add: bind_def)
+  note th = a[OF sa, simplified b[THEN conjunct1]]
+  from th[THEN SpecTop_focus] show "s' \<in> \<S_S> T" using b by (blast intro: LooseStateTy_upgrade)
+  from th[THEN SpecTop_facts] show "PROP L" .
+qed
+
+theorem start_construction: "CodeBlock s a S begin_proc_ctx \<Longrightarrow> \<^bold>c\<^bold>u\<^bold>r\<^bold>r\<^bold>e\<^bold>n\<^bold>t s \<B_r>\<B_e>\<^bold>s\<B_u>\<B_l>\<B_t>\<^bold>s \<^bold>i\<^bold>n (S \<flower> Void) \<^bold>w\<^bold>i\<^bold>t\<^bold>h \<^bold>f\<^bold>a\<^bold>c\<^bold>t\<^bold>s: (PROP NoFact)"
+  unfolding begin_proc_ctx_def CodeBlock_def CurrentConstruction_def by (rule SpecTop_I; (rule NoFact)?) auto
+
+theorem finish_construction: "\<medium_left_bracket>\<And>a s. CodeBlock s a S f \<Longrightarrow> \<^bold>c\<^bold>u\<^bold>r\<^bold>r\<^bold>e\<^bold>n\<^bold>t s \<B_r>\<B_e>\<^bold>s\<B_u>\<B_l>\<B_t>\<^bold>s \<^bold>i\<^bold>n (T \<flower> R) \<^bold>w\<^bold>i\<^bold>t\<^bold>h \<^bold>f\<^bold>a\<^bold>c\<^bold>t\<^bold>s: PROP L \<medium_right_bracket>
+  \<Longrightarrow> f' = f \<nuInstrComp> end_proc_ctx \<Longrightarrow> \<^bold>p\<^bold>r\<^bold>o\<^bold>c f' \<llangle> S \<longmapsto> T \<rrangle>"
+    unfolding PropBlock_def CodeBlock_def
+proof
+  assume rule:"(\<And>a s. a \<in> S \<and> f a = s \<and> s \<noteq> SNeg \<Longrightarrow> \<^bold>c\<^bold>u\<^bold>r\<^bold>r\<^bold>e\<^bold>n\<^bold>t s \<B_r>\<B_e>\<^bold>s\<B_u>\<B_l>\<B_t>\<^bold>s \<^bold>i\<^bold>n (T \<flower> R) \<^bold>w\<^bold>i\<^bold>t\<^bold>h \<^bold>f\<^bold>a\<^bold>c\<^bold>t\<^bold>s: PROP L)"
+    and def: "f' = f \<nuInstrComp> end_proc_ctx"
+  fix a show "a \<in> S \<longrightarrow> f' a \<in> \<S> T " unfolding def proof
+    assume a: "a \<in> S"
+    moreover note rule[of a "f a", unfolded CurrentConstruction_def, simplified, THEN SpecTop_focus] 
+    ultimately show "(f \<nuInstrComp> end_proc_ctx) a \<in> \<S> T" unfolding instr_comp_def bind_def end_proc_ctx_def
+      using LooseStateTy_introByStrict by (cases "f a") auto
+  qed
+qed
+
+definition ParamTag :: " 'a \<Rightarrow> prop" ("\<^bold>p\<^bold>a\<^bold>r\<^bold>a\<^bold>m") where "\<^bold>p\<^bold>a\<^bold>r\<^bold>a\<^bold>m x \<equiv> Trueprop True"
+lemma ParamTag_E: "PROP \<^bold>p\<^bold>a\<^bold>r\<^bold>a\<^bold>m x" unfolding ParamTag_def using TrueI .
+  \<comment>\<open>A tag used to indicate a parameter should be specified during application. It retains the order of the parameters to be specified.
+  For example, "@{prop "\<And>bit_width value. PROP \<^bold>p\<^bold>a\<^bold>r\<^bold>a\<^bold>m bit_width \<Longrightarrow> PROP \<^bold>p\<^bold>a\<^bold>r\<^bold>a\<^bold>m value \<Longrightarrow> \<^bold>p\<^bold>r\<^bold>o\<^bold>c const_nat \<llangle> R \<longmapsto> (value \<tycolon> NuNat bit_width) \<rrangle>"},
+    the first parameter `?bit_width` will be specified first and then the "?value".\<close>
 
 end
-  
