test.thy
@@ -1,0 +1,7 @@
+theory test
+  imports Main
+begin
+text\<open>interesting\<close>
+definition "hh = (o)"
+\<comment>\<open>hahaha\<close>
+end
