ROOT
@@ -1,0 +1,9 @@
+session NuSystem = HOL +
+  description "
+    \<nu>-system.
+  "
+  options [document = pdf, document_output = "output"]  
+  theories
+    test
+  document_files
+    "root.tex"
